{
 "cells": [
  {
   "cell_type": "markdown",
   "metadata": {},
   "source": [
    "# Conditional Probability"
   ]
  },
  {
   "cell_type": "markdown",
   "metadata": {},
   "source": [
    "# Basic Concepts"
   ]
  },
  {
   "cell_type": "markdown",
   "metadata": {},
   "source": [
    "## Definition\n",
    "$$ P(A|B) = \\frac {P(A,B)}{P(B)} $$\n",
    "Basically, when $P(A) \\ne 0$, $P(B) \\ne 0$:\n",
    "$$P(A) = \\sum_B P(A|B)P(B) = \\sum_B P(A,B)$$\n",
    "$$ 1 = \\sum_A P(A|B) = \\sum_A \\frac {P(A,B)}{P(B)} = \\frac {\\sum_A P(A,B)}{P(B)} = \\frac {P(B)}{P(B)}$$"
   ]
  },
  {
   "cell_type": "markdown",
   "metadata": {},
   "source": [
    "## Factorization\n",
    "Factorize the probability in a trail, for example\n",
    "$$ P(A,B,C) = P(A|B,C)P(B|C)P(C) $$\n",
    "This factorization correspond a Bayesian map:  \n",
    "$$ C \\to B \\to A $$\n",
    "$$ C \\to A $$"
   ]
  },
  {
   "cell_type": "markdown",
   "metadata": {},
   "source": [
    "## Statistical independence\n",
    "Events $A$ and $B$ are defined to be statistically independent if $ P(A,B)=P(A)P(B) $, so we have:\n",
    "$$ P(A|B) = P(A) $$\n",
    "$$ P(B|A) = P(B) $$\n",
    "The notations of independence is $ P \\models A \\perp B$, where $\\models$ means \"satisfy\", and $\\perp$ means \"independent\".\n",
    "\n",
    "For random variables $X$,$Y$, $ P \\models X \\perp Y$, similarly, we have:\n",
    "$$ P(X,Y) = P(X)P(Y) $$\n",
    "$$ P(X|Y) = P(X) $$\n",
    "$$ P(Y|X) = P(Y) $$\n",
    "\n",
    "## Conditional Independence\n",
    "For (sets of) random variables $X$,$Y$,$Z$, $P \\models (X \\perp Y | Z)$ if:\n",
    "$$ P(X,Y|Z) = P(X|Z)P(Y|Z)$$\n",
    "$$ P(X|Y,Z) = P(X|Z) $$\n",
    "$$ P(Y|X,Z) = P(Y|Z) $$\n",
    "The conditional independence means that the $X$ and $Y$ are conditionally independent given $Z$, but reminder that this statement may not work given another variables other than $Z$.\n"
   ]
  },
  {
   "cell_type": "markdown",
   "metadata": {},
   "source": [
    "## Bayes' theorem\n",
    "$$ P(A|B)=\\frac{P(B|A)P(A)}{P(B)}$$\n",
    "Actually, they follow as the form $ P(A,B)=P(A|B)P(B) = P(B|A)P(A)$. In general, it cannot be assumed that $P(A|B) \\approx P(B|A)$.\n",
    "\n",
    "$$ \\frac {P(B|A)}{P(A|B)} = \\frac {P(B)}{P(A)} $$\n",
    "\n",
    "Sometimes, for $A$ is a binary variable, we can write the probability in alternative form as $ P(B) = P(B|A)P(A) + P(B|\\overline{A})P(\\overline{A})$, thus we have:\n",
    "$$ P(A|B)=\\frac{P(B|A)P(A)} {P(B|A)P(A) + P(B|\\overline{A})P(\\overline{A})}$$\n",
    "\n",
    "Often, for some partition ${A_j}$ of the sample space, the event space is given or conceptualized in terms of $P(A_j)$ and $P(B|A_j)$. It is then useful to compute $P(B)$ using the law of total probability $P(B) = \\sum_j P(B|A_j)P(A_j)$:\n",
    "$$ P(A_i|B) = \\frac{P(B|A_i)P(A_i)}{\\sum_j P(B|A_j)P(A_j)}$$"
   ]
  },
  {
   "cell_type": "markdown",
   "metadata": {},
   "source": [
    "# Multi-conditional probability\n",
    "$$ P(Y|X_1,X_2) = \\frac {P(Y,X_1,X_2)} {P(X_1,X_2)}$$\n",
    "$$ P(Y_1,Y_2|X) = \\frac {P(Y_1,Y_2,X)} {P(X)} $$"
   ]
  },
  {
   "cell_type": "markdown",
   "metadata": {},
   "source": [
    "## Influence Flow\n",
    "$$ P(X_1|X_2) = \\frac {P(X_1,X_2)} {P(X_2)} = \\frac{P(Y,X_1,X_2)} {P(Y|X_1,X_2)P(X_2)}$$\n",
    "$X_1$ and $X_2$ are independent, but conditionally dependent given $Y$, which activates the V-structure, $ P(X_1|X_2) \\ne P(X_1) $."
   ]
  },
  {
   "cell_type": "markdown",
   "metadata": {},
   "source": [
    "## D-separation\n",
    "Definition: $X$ and $Y$ are d-separated in G given $Z$ if there is no active trail in G (likely, V-structure) betweeb $X$ and $Y$ given $Z$, notation: $d-sep_G(X,Y|Z)$.\n",
    "\n",
    ">Theorem: If $P$ factorizes over $G$, and $d-sep_G(X,Y|Z)$ then $P$ satisfies $(X \\perp Y |Z)$\n",
    "\n",
    "For example, $ P(D,I,G,S,L) = P(D)P(I)P(G|D,I)P(S|I)P(L|G)$, so\n",
    "$$ P(D,S) = \\sum_{G,L,I} P(D)P(I)P(G|D,I)P(S|I)P(L|G) $$\n",
    "$$ P(D,S) = \\sum_I P(D)P(I)P(S|I) \\sum_G (P(G|D,I)\\sum_L P(L|G)) $$\n",
    "\n",
    "we have $1 = \\sum_L P(L|G)$, $1 = \\sum_G P(G|D,I)$, and $P(S) = \\sum_I P(I)P(S|I)$, so \n",
    "\n",
    "$$ P(D,S) = P(D)P(S) $$\n",
    "Thus, $D$ and $S$ are independent.\n",
    "\n",
    ">Any node is d-separated from its non-descendants given its parents"
   ]
  },
  {
   "cell_type": "markdown",
   "metadata": {},
   "source": [
    "## I-maps\n",
    "+ Definition: d-separation in $G \\to P$ satisfies corresonding independence statement  $I(G)={(X \\perp Y|Z):d-sep_G(X,Y|Z)}$.\n",
    "+ Definition: If $P$ satisfies $I(G)$, we say that $G$ is an I-map(independency map) of $P$.\n",
    "\n",
    "> If $P$ factorizes over $G$, then $G$ is an I-map for $P$, reversely, if $G$ is an I-map for $P$, then $P$ factorizes over $G$.\n",
    "\n",
    "Basically, according to the chain rule, the factorization shall be written as:\n",
    "$$P(D,I,G,S,L)=P(D)P(I|D)P(G|D,I)P(S|D,I,G)P(L|D,I,G,S)$$\n",
    "because $P(S|D,I,G) = P(S|I)$, $P(L|D,I,G,S) = P(L|G)$, $P(I) = P(I|D)$\n",
    "$$P(D,I,G,S,L)=P(D)P(I|D)P(G|D,I)P(S|I)P(L|G)$$"
   ]
  },
  {
   "cell_type": "markdown",
   "metadata": {},
   "source": [
    "## Beyasian Network"
   ]
  },
  {
   "cell_type": "code",
   "execution_count": null,
   "metadata": {
    "collapsed": true
   },
   "outputs": [],
   "source": []
  }
 ],
 "metadata": {
  "anaconda-cloud": {},
  "kernelspec": {
   "display_name": "Python [Root]",
   "language": "python",
   "name": "Python [Root]"
  },
  "language_info": {
   "codemirror_mode": {
    "name": "ipython",
    "version": 2
   },
   "file_extension": ".py",
   "mimetype": "text/x-python",
   "name": "python",
   "nbconvert_exporter": "python",
   "pygments_lexer": "ipython2",
   "version": "2.7.12"
  }
 },
 "nbformat": 4,
 "nbformat_minor": 0
}
